\text{Dadas as funções $f\left( x\right) = 3x - 1$ e $g\left( x \right) = x^{2} + x - 1$, determine: $fog\left( x\right)$} \\ \\

\text{$\bbox[#CC3333]{\color{white}{f\left( x \right) = 3x - 1}}$ e $\bbox[#CC3333]{\color{white}g\left( x \right) = x^{2} + x - 1}$} \\ \\

fog\left( x \right) = f\left( g\left( x \right) \right) = f\left( x^{2} + x  - 1 \right) = 3 \cdot

\left( x^{2} + x - 1 \right) - 1 = 3x^{2} + 3x - 3 - 1  \\ \\

\bbox[#CC3333]{\color{white}{fog\left( x \right) = 3x^{2} + 3x - 4}}

